Source/DafnyRuntime/DafnyRuntimeDafny/src/sequence.dfy
@@ -1,157 +1,327 @@
-include "../../../../Test/libraries/src/JSON/Stacks.dfy"
 include "../../../../Test/libraries/src/Collections/Sequences/Seq.dfy"
 include "../../../../Test/libraries/src/Math.dfy"
 
 include "array.dfy"
+include "frames.dfy"
 
 module {:options "/functionSyntax:4"} MetaSeq {
 
   import Math
   import Seq
 
-  import opened Stacks
+  import opened Frames
   import opened Arrays
 
   // TODO: static analysis to assert that all methods that are called directly from Dafny syntax
   // (e.g. s[i] -> s.Select(i)) have `modifies {}` (implicitly or explicitly).
   // TODO: Would also be good to assert that seq<T> is only used in specifications.
-  datatype SeqExpr<T> = 
-    | Empty
-    | Direct(a: seq<T>)
-    | ConcatBoth(left: SeqExpr<T>, right: SeqExpr<T>, length: nat)
-    | Lazy(ghost value: seq<T>, ghost boxSize: nat,
-           exprBox: AtomicBox<SeqExpr<T>>, length: nat)
-  {
+  // TODO: Align terminology between length/size/etc.
+  // TODO: How to deal
+  trait SeqExpr<T> extends Validatable {
+   
     ghost predicate Valid()
-      decreases Size(), 0
-    {
-      match this
-      case ConcatBoth(left, right, length) => 
-        && left.Valid()
-        && right.Valid()
-        && left.Length() + right.Length() == length
-      case Lazy(value, size, exprBox, length) => 
-        && length == |value|
-        && exprBox.inv == ((e: SeqExpr<T>) => 
-          && e.Size() < size
-          && e.Valid() 
-          && e.Value() == value)
-      case _ => true
-    }
-
-    ghost function Size(): nat {
-      match this {
-        case ConcatBoth(left, right, _) => 1 + left.Size() + right.Size()
-        case Lazy(_, boxSize, _, _) => 1 + boxSize
-        case _ => 1
-      }
-    }
-
-    function Length(): nat {
-      match this
-      case Empty => 0
-      case Direct(a) => |a|
-      case ConcatBoth(_, _, length) => length
-      case Lazy(_, _, _, length) => length
-    }
-
-    function At(i: nat): T 
+      reads this, Repr
+      decreases Repr, 0
+      ensures Valid() ==> this in Repr
+    
+    ghost function Size(): nat
       requires Valid()
-      requires i < Length()
-    {
-      Value()[i]
-    }
+      reads this, Repr
+      decreases Repr, 1
+
+    function Length(): nat 
+      requires Valid() 
+      reads Repr
+      decreases Repr, 1
+
+    function Depth(): nat
+
+    ghost function Value(): seq<T> 
+      requires Valid()
+      reads this, Repr
+      decreases Repr, 2
+      ensures |Value()| == Length()
+
+    method ToArray() returns (ret: InitializedArray<T>)
+      requires Valid()
+      decreases Size(), 2
+      ensures ret.Valid()
+      ensures ret.Value() == Value()
 
     method Concatenate(s: SeqExpr<T>) returns (ret: SeqExpr<T>)
       requires Valid()
       requires s.Valid()
       ensures ret.Valid()
     {
-      var c := ConcatBoth(this, s, Length() + s.Length());
+      var c := new Concat(this, s);
+      ret := new Lazy(c);
+    }
+  }
 
-      ghost var value := c.Value();
-      ghost var size := 1 + c.Size();
-      ghost var inv := ((e: SeqExpr<T>) => 
-          && e.Size() < size
-          && e.Valid() 
-          && e.Value() == value);
-      var box := new AtomicBox(inv, c);
-      return Lazy(value, size, box, c.Length());
+  class Direct<T> extends SeqExpr<T> {
+    const value: InitializedArray<T>
+
+    ghost predicate Valid()
+      reads this, Repr
+      decreases Repr, 0
+      ensures Valid() ==> this in Repr
+    {
+      && this in Repr
+      && ValidComponent(value.a)
+      && value.Valid()
     }
 
-    function Value(): seq<T> 
+    constructor(value: InitializedArray<T>) 
+      requires value.Valid()
+      ensures Valid()
+      ensures fresh(Repr - value.a.Repr)
+    {
+      this.value := value;
+
+      Repr := {this} + value.a.Repr;
+    }
+
+    ghost function Size(): nat 
       requires Valid()
-      decreases Size(), 2
+      reads this, Repr
+      decreases Repr, 1
+    {
+      1
+    }
+
+    function Depth(): nat {
+      1
+    }
+
+    function Length(): nat 
+      requires Valid() 
+      reads Repr 
+      decreases Repr, 1
+    {
+      value.a.Length()
+    }
+
+    ghost function Value(): seq<T> 
+      requires Valid()
+      reads this, Repr
+      decreases Repr, 2
       ensures |Value()| == Length()
     {
-      match this
-      case Empty => []
-      case Direct(a) => a
-      case ConcatBoth(left, right, _) => left.Value() + right.Value()
-      case Lazy(value, _, _, _) => value
-    } by method {
-      match this
-      case Empty => return [];
-      case Direct(a) => return a;
-      case ConcatBoth(left, right, length) => {
-        var builder := new SeqBuilder<T>(length);
-        var toAppendAfter := new Stack<SeqExpr<T>>(Empty);
-        AppendValue(builder, toAppendAfter);
-        return builder.Value();
-      }
-      case Lazy(_, _, seqExpr, _) => {
-        var expr := exprBox.Get();
-        var value := expr.Value();
-        exprBox.Put(Direct(value));
-        return value;
-      }
+      value.Value()
     }
 
-    method {:tailrecursion} AppendValue(builder: SeqBuilder<T>, toAppendAfter: Stack<SeqExpr<T>>)
+    method ToArray() returns (ret: InitializedArray<T>)
+      requires Valid()
+      decreases Size(), 2
+      ensures ret.Valid()
+      ensures ret.Value() == Value()
+    {
+      return value;
+    }
+  }
+
+  class Concat<T> extends SeqExpr<T> {
+    const left: SeqExpr<T>
+    const right: SeqExpr<T>
+    const length: nat
+    const depth: nat
+
+    ghost predicate Valid() 
+      reads this, Repr
+      decreases Repr, 0
+      ensures Valid() ==> this in Repr
+    {
+      && this in Repr
+      && ValidComponent(left)
+      && ValidComponent(right)
+      && length == left.Length() + right.Length()
+      && depth == 1 + Math.Max(left.Depth(), right.Depth())
+    }
+
+    constructor(left: SeqExpr<T>, right: SeqExpr<T>) 
+      requires left.Valid()
+      requires right.Valid()
+      ensures Valid()
+      ensures fresh(Repr - left.Repr - right.Repr)
+    {
+      this.left := left;
+      this.right := right;
+      this.length := left.Length() + right.Length();
+      this.depth := 1 + Math.Max(left.Depth(), right.Depth());
+
+      Repr := {this} + left.Repr + right.Repr;
+    }
+
+    ghost function Size(): nat
+      requires Valid()
+      reads this, Repr
+      decreases Repr, 1
+    {
+      1 + left.Size() + right.Size()
+    }
+
+    function Depth(): nat {
+      depth
+    }
+
+    function Length(): nat 
+      requires Valid() 
+      reads Repr 
+      decreases Repr, 1
+    {
+      length
+    }
+
+    ghost function Value(): seq<T> 
+      requires Valid()
+      reads this, Repr
+      decreases Repr, 2
+      ensures |Value()| == Length()
+    {
+      var result := left.Value() + right.Value();
+      assert |result| == length;
+      assert length == Length();
+      result
+    }
+
+    method ToArray() returns (ret: InitializedArray<T>)
+      requires Valid()
+      decreases Size(), 2
+      ensures ret.Valid()
+      ensures ret.Value() == Value()
+    {
+      var builder := new ResizableArray<T>(length);
+      var toAppendAfter := new ResizableArray<SeqExpr<T>>(depth);
+      AppendValue(builder, toAppendAfter);
+      return InitializedArray(builder.storage);
+    }
+
+    method {:tailrecursion} AppendValue(builder: ResizableArray<T>, toAppendAfter: ResizableArray<SeqExpr<T>>)
       requires Valid()
       requires builder.Valid()
-      requires toAppendAfter.Valid?()
-      requires forall e <- toAppendAfter.Repr :: e.Valid()
-      requires builder.Remaining() == |Value()| + |ConcatValueOnStack(toAppendAfter.Repr)|
-      requires builder.Repr !! {toAppendAfter, toAppendAfter.data}
-      modifies builder.Repr, toAppendAfter, toAppendAfter.data
-      decreases Size() + SizeSum(toAppendAfter.Repr)
+      requires toAppendAfter.Valid()
+      requires forall e <- toAppendAfter.Value() :: e.Valid()
+      requires builder.Remaining() == |Value()| + |ConcatValueOnStack(toAppendAfter.Value())|
+      requires builder.Repr !! toAppendAfter.Repr
+      modifies builder.Repr, toAppendAfter.Repr
+      decreases Size() + SizeSum(toAppendAfter.Value())
       ensures builder.Valid()
-      ensures builder.Value() == old(builder.Value()) + Value() + ConcatValueOnStack(old(toAppendAfter.Repr));
+      ensures builder.Value() == old(builder.Value()) + Value() + ConcatValueOnStack(old(toAppendAfter.Value()));
     {
-      match this {
-        case Empty =>
-          if 0 < toAppendAfter.size {
-            var next := toAppendAfter.Pop();
-            LemmaConcatValueOnStackWithTip(toAppendAfter.Repr, next);
-            next.AppendValue(builder, toAppendAfter);
-          }
-        case Direct(a) => {
-          builder.Append(a);
-          if 0 < toAppendAfter.size {
-            var next := toAppendAfter.Pop();
-            LemmaConcatValueOnStackWithTip(toAppendAfter.Repr, next);
-            next.AppendValue(builder, toAppendAfter);
-          }
-        }
-        case ConcatBoth(left, right, _) => {
-          :- expect toAppendAfter.Push(right);
-          LemmaConcatValueOnStackWithTip(old(toAppendAfter.Repr), right);
-          assert SizeSum(toAppendAfter.Repr) == old(SizeSum(toAppendAfter.Repr)) + right.Size();
-          left.AppendValue(builder, toAppendAfter);
-        }
-        case Lazy(_, _, exprBox, _) => {
-          var expr := exprBox.Get();
-          expr.AppendValue(builder, toAppendAfter);
-        }
-      }
+      // TODO: Optimized version
+      // match this {
+      //   case Direct(a) => {
+      //     builder.Append(a);
+      //     if 0 < toAppendAfter.size {
+      //       var next := toAppendAfter.RemoveLast();
+      //       LemmaConcatValueOnStackWithTip(toAppendAfter.Value(), next);
+      //       next.AppendValue(builder, toAppendAfter);
+      //     }
+      //   }
+      //   case ConcatBoth(left, right, _, _) => {
+      //     toAppendAfter.AddLast(right);
+      //     LemmaConcatValueOnStackWithTip(old(toAppendAfter.Value()), right);
+      //     assert SizeSum(toAppendAfter.Value()) == old(SizeSum(toAppendAfter.Value())) + right.Size();
+      //     left.AppendValue(builder, toAppendAfter);
+      //   }
+      //   case Lazy(_, _, exprBox, _, _) => {
+      //     var expr := exprBox.Get();
+      //     expr.AppendValue(builder, toAppendAfter);
+      //   }
+      // }
+    }
+  }
+
+  class Lazy<T> extends SeqExpr<T> {
+    ghost const value: seq<T>
+    ghost const size: nat
+    const exprBox: AtomicBox<SeqExpr<T>>
+    const length: nat
+    const depth: nat
+
+    ghost predicate Valid() 
+      reads this, Repr
+      decreases Repr, 0
+      ensures Valid() ==> this in Repr
+    {
+      && this in Repr
+      && length == |value|
+      && exprBox.inv == ((e: SeqExpr<T>) reads e => 
+        && e.Size() < size
+        && e.Depth() < depth
+        && e.Valid() 
+        && e.Value() == value)
+    }
+
+    constructor(wrapped: SeqExpr<T>) 
+      requires wrapped.Valid()
+      ensures Valid()
+      ensures fresh(Repr)
+    {
+      var depth := 1 + wrapped.Depth();
+      var value := wrapped.Value();
+      var size := 1 + wrapped.Size();
+      ghost var inv := ((e: SeqExpr<T>) => 
+          && e.Size() < size
+          && e.Depth() < depth
+          && e.Valid() 
+          && e.Value() == value);
+      this.exprBox := new AtomicBox(inv, wrapped);
+
+      this.depth := depth;
+      this.value := value;
+      this.size := size;
+    }
+
+    ghost function Size(): nat 
+      requires Valid()
+      reads this, Repr
+      decreases Repr, 1
+    {
+      size
+    }
+
+    function Depth(): nat {
+      depth
+    }
+
+    function Length(): nat 
+      requires Valid() 
+      reads Repr
+      decreases Repr, 1
+    {
+      length
+    }
+    
+    ghost function Value(): seq<T> 
+      requires Valid()
+      reads this, Repr
+      decreases Repr, 2
+      ensures |Value()| == Length()
+    {
+      assert |value| == Length();
+      value
+    }
+
+    method ToArray() returns (ret: InitializedArray<T>)
+      requires Valid()
+      decreases Size(), 2
+      ensures ret.Valid()
+      ensures ret.Value() == Value()
+    {
+      var expr := exprBox.Get();
+      var a := expr.ToArray();
+      var direct := new Direct(a);
+      exprBox.Put(direct);
+      return a;
     }
   }
 
   ghost function ConcatValueOnStack<T>(s: seq<SeqExpr<T>>): seq<T>
+    reads (set e <- s, o <- e.Repr :: o)
     requires (forall e <- s :: e.Valid())
   {
-    var valueFn := (e: SeqExpr<T>) requires e.Valid() => e.Value();
+    var valueFn := (e: SeqExpr<T>) requires e.Valid() reads e, e.Repr => e.Value();
     Seq.Flatten(Seq.Map(valueFn, Seq.Reverse(s)))
   }
 
@@ -160,7 +330,7 @@ module {:options "/functionSyntax:4"} MetaSeq {
     requires x.Valid()
     ensures ConcatValueOnStack(s + [x]) == x.Value() + ConcatValueOnStack(s)
   {
-    var valueFn := (e: SeqExpr<T>) requires e.Valid() => e.Value();
+    var valueFn := (e: SeqExpr<T>) reads e, e.Repr requires e.Valid() => e.Value();
     calc {
       ConcatValueOnStack(s + [x]);
       Seq.Flatten(Seq.Map(valueFn, Seq.Reverse(s + [x])));
@@ -173,7 +343,10 @@ module {:options "/functionSyntax:4"} MetaSeq {
     }
   }
 
-  ghost function SizeSum<T>(s: seq<SeqExpr<T>>): nat {
+  ghost function SizeSum<T>(s: seq<SeqExpr<T>>): nat 
+    reads set e <- s, o <- e.Repr :: o
+    requires forall e <- s :: e.Valid()
+  {
     if |s| == 0 then 
       0 
     else
@@ -181,8 +354,7 @@ module {:options "/functionSyntax:4"} MetaSeq {
       SizeSum(s[..last]) + s[last].Size()
   }
 
-  // TODO: Make this an extern. How to monomorphize?
-  class SeqBuilder<T> extends Validatable {
+  class ResizableArray<T> extends Validatable {
     const storage: Array<T>
     var size: nat
 
@@ -207,6 +379,13 @@ module {:options "/functionSyntax:4"} MetaSeq {
       Repr := {this} + storage.Repr;
     }
 
+    ghost function Value(): seq<T>
+      requires Valid()
+      reads this, Repr
+    {
+      seq(size, i requires 0 <= i < size && Valid() reads this, Repr => storage.Read(i))
+    }
+
     ghost function Remaining(): nat
       requires Valid()
       reads this, Repr
@@ -214,23 +393,41 @@ module {:options "/functionSyntax:4"} MetaSeq {
       storage.Length() - size
     }
 
-    method Append(t: seq<T>) 
+    method AddLast(t: T) 
       requires Valid()
-      requires size + |t| <= storage.Length()
+      requires size + 1 <= storage.Length()
       modifies Repr
       ensures ValidAndDisjoint()
-      ensures Value() == old(Value()) + t
-      ensures Remaining() == old(Remaining()) - |t|
+      ensures Value() == old(Value()) + [t]
+      ensures Remaining() == old(Remaining()) - 1
     {
-      storage.WriteRange(size, t);
-      size := size + |t|;
+      storage.Write(size, t);
+      size := size + 1;
     }
 
-    function Value(): seq<T>
+    method RemoveLast() returns (t: T) 
       requires Valid()
-      reads this, Repr
+      requires 0 < size
+      modifies Repr
+      ensures ValidAndDisjoint()
+      ensures Value() == old(Value())[..size]
+      ensures Remaining() == old(Remaining()) + 1
     {
-      seq(size, i requires 0 <= i < size && Valid() reads this, Repr => storage.Read(i))
+      t := storage.Read(size - 1);
+      size := size - 1;
+    }
+
+    method Append(other: InitializedArray<T>) 
+      requires Valid()
+      requires other.Valid()
+      requires size + other.a.Length() <= storage.Length()
+      modifies Repr
+      ensures ValidAndDisjoint()
+      ensures Value() == old(Value()) + other.Value()
+      ensures Remaining() == old(Remaining()) - other.a.Length()
+    {
+      storage.WriteRangeArray(size, other.a, 0, other.a.Length());
+      size := size + other.a.Length();
     }
   }
 
